Impl card_toFinset

ErdosStoneSimonovits/Data/Sym/Sym2.lean
@@ -11,7 +11,7 @@ section ToMultiset
 /-- Map an unordered pair to an unordered list. -/
 def toMultiset {α : Type*} (z : Sym2 α) : Multiset α := by
   refine Sym2.lift ?_ z
-  use Multiset.ofList [·, ·]
+  use (Multiset.ofList [·, ·])
   simp [List.Perm.swap]
 
 /-- Mapping an unordered pair to an unordered list produces a multiset of size `2`. -/
@@ -20,8 +20,9 @@ lemma card_toMultiset {α : Type*} (z : Sym2 α) : z.toMultiset.card = 2 := by
   simp [Sym2.toMultiset]
 
 /-- The members of an unordered pair are members of the corresponding unordered list. -/
+@[simp]
 theorem mem_toMultiset {α : Type*} {x : α} {z : Sym2 α} :
-    x ∈ z ↔ x ∈ (z.toMultiset : Multiset α) := by
+    x ∈ (z.toMultiset : Multiset α) ↔ x ∈ z := by
   induction z
   simp [Sym2.toMultiset]
 
@@ -29,30 +30,37 @@ end ToMultiset
 
 section ToFinset
 
+variable [DecidableEq α]
+
 /-- Map an unordered pair to a finite set. -/
-abbrev toFinset [DecidableEq α] (z : Sym2 α) : Finset α :=
-  (z.toMultiset : Multiset α).toFinset
+def toFinset (z : Sym2 α) : Finset α := (z.toMultiset : Multiset α).toFinset
 
 /-- The members of an unordered pair are members of the corresponding finite set. -/
-theorem mem_toFinset [DecidableEq α] {x : α} {z : Sym2 α} : x ∈ z ↔ x ∈ z.toFinset := by
-  rw [Sym2.mem_toMultiset, Multiset.mem_toFinset]
+@[simp]
+theorem mem_toFinset {x : α} {z : Sym2 α} : x ∈ z.toFinset ↔ x ∈ z := by
+  rw [← Sym2.mem_toMultiset, Sym2.toFinset, Multiset.mem_toFinset]
 
-lemma toFinset_mk_eq [DecidableEq α] {x y : α} : s(x, y).toFinset = {x, y} := by
-  ext; simp [← Sym2.mem_toFinset, ← Sym2.mem_iff, Sym2.mem_toMultiset]
+lemma toFinset_mk_eq {x y : α} : s(x, y).toFinset = {x, y} := by
+  ext; simp [←Sym2.mem_toFinset, ←Sym2.mem_iff, Sym2.mem_toMultiset]
 
-/-- The size of the finite set corresponding to an unordered pair on the diagonal is `1`. -/
-theorem card_toFinset_of_isDiag [DecidableEq α] (z : Sym2 α) (h : z.IsDiag) :
-    #(z : Sym2 α).toFinset = 1 := by
+/-- Mapping an unordered pair on the diagonal to a finite set produces a finset of size `1`. -/
+theorem card_toFinset_of_isDiag (z : Sym2 α) (h : z.IsDiag) : #(z : Sym2 α).toFinset = 1 := by
   induction z
   rw [Sym2.mk_isDiag_iff] at h
   simp [Sym2.toFinset_mk_eq, h]
 
-/-- The size of the finite set corresponding to an unordered pair off the diagonal is `2`. -/
-theorem card_toFinset_of_not_isDiag [DecidableEq α] (z : Sym2 α) (h : ¬z.IsDiag) :
-    #(z : Sym2 α).toFinset = 2 := by
+/-- Mapping an unordered pair off the diagonal to a finite set produces a finset of size `2`. -/
+theorem card_toFinset_of_not_isDiag (z : Sym2 α) (h : ¬z.IsDiag) : #(z : Sym2 α).toFinset = 2 := by
   induction z
   rw [Sym2.mk_isDiag_iff] at h
   simp [Sym2.toFinset_mk_eq, h]
+
+/-- Mapping an unordered pair to a finite set produces a finset of size `1` if the pair is on the
+diagonal, else of size `2` if the pair is off the diagonal. -/
+theorem card_toFinset (z : Sym2 α) : #(z : Sym2 α).toFinset = if z.IsDiag then 1 else 2 := by
+  by_cases h : z.IsDiag
+  · simp [card_toFinset_of_isDiag z h, h]
+  · simp [card_toFinset_of_not_isDiag z h, h]
 
 end ToFinset
 
